Refactor and enhance the AlgEffectus.Core module
- Updated pretty-printing for `Value` to use `toString` for variable names.
- Refactored renaming functions to improve termination proofs and ensure proper handling of names.
- Introduced scoped notation for single and multi-step reductions in semantics.
- Improved substitution functions to ensure proper handling of alpha-renaming and termination.
- Enhanced syntax definitions with size calculations for values, computations, and handlers.
- Added a new TypeSafety module to formalize preservation and progress theorems for the type system.
- Introduced a Typing module to define the core type system for algebraic effects and handlers.
- Improved overall structure and readability of the codebase.

src/AlgEffectus/Core/Rename.lean
@@ -1,43 +1,134 @@
 import AlgEffectus.Core.Syntax
 
+-- import LeanCopilot
+import aesop
+
 open AlgEffectus.Core
 
 mutual
-  partial def renameValue (old new : Name) : Value → Value
-  | v@(Value.varV n)     => if n = old then Value.varV new else v
-  | Value.funV x body    =>
-      let (x', body') :=
-        if x = old then (x, body) else (x, renameComp old new body)
-      Value.funV x' body'
-  | Value.handV h        => Value.handV (renameHandler old new h)
-  | v                    => v
+  def renameValue (old new : Name) : Value → Value
+  | v@(Value.varV n)  => if n = old then Value.varV new else v
+  | Value.funV x body =>
+    let (x', body') :=
+      if x = old then (x, body) else (x, renameComp old new body)
+    Value.funV x' body'
+  | Value.handV h    => Value.handV (renameHandler old new h)
+  | v                => v
 
-  partial def renameHandler (old new : Name) : Handler → Handler
+  termination_by
+    v => sizeOfValue v
+  decreasing_by
+    repeat dsimp [sizeOfValue]; simp
+
+  def renameHandler (old new : Name) : Handler → Handler
   | Handler.mk rb rc opcs =>
-      let rb' := rb
-      let rc' := if rb = old then rc else renameComp old new rc
-      let opcs' := opcs.map fun (op,x,k,c) =>
-        let x' := x; let k' := k
-        let c' := if x = old ∨ k = old then c else renameComp old new c
-        (op,x',k',c')
-      Handler.mk rb' rc' opcs'
+    let rb' := rb
+    let rc' := if rb = old then rc else renameComp old new rc
+    let opcs' := opcs.map fun opcl =>
+      let (op,x,k,c) := opcl
+      -- When proving termination, changing `opcl.snd.snd.snd` to `c` causes issues.
+      let c' := if x = old ∨ k = old then c else renameComp old new opcl.snd.snd.snd
+      (op, x, k, c')
 
-  partial def renameComp (old new : Name) : Computation → Computation
+    Handler.mk rb' rc' opcs'
+
+  termination_by
+    h => sizeOfHandler h
+  decreasing_by
+    repeat dsimp [sizeOfComp, sizeOfHandler]; simp +arith
+    rename_i h_mem
+    have h₁ : sizeOfComp opcl.snd.snd.snd ≤ sizeOfOpClauses opcs := by
+      induction h_mem with
+      | head _ => dsimp [sizeOfOpClauses]; simp
+      | tail _ _ ih₁=>
+        simp [sizeOfOpClauses, Nat.le_trans ih₁]
+    apply Nat.le_trans h₁; simp +arith
+
+  def renameComp (old new : Name) : Computation → Computation
   | Computation.retC v              => Computation.retC (renameValue old new v)
   | Computation.callC op arg k body =>
-      let arg' := renameValue old new arg
-      let body' := if k = old then body else renameComp old new body
-      Computation.callC op arg' k body'
+    let arg' := renameValue old new arg
+    let body' := if k = old then body else renameComp old new body
+    Computation.callC op arg' k body'
   | Computation.seqC x c1 c2        =>
-      let c1' := renameComp old new c1
-      let c2' := if x = old then c2 else renameComp old new c2
-      Computation.seqC x c1' c2'
+    let c1' := renameComp old new c1
+    let c2' := if x = old then c2 else renameComp old new c2
+    Computation.seqC x c1' c2'
   | Computation.ifC b t e           =>
-      Computation.ifC (renameValue old new b)
-                      (renameComp old new t)
-                      (renameComp old new e)
+    Computation.ifC (renameValue old new b)
+                    (renameComp old new t)
+                    (renameComp old new e)
   | Computation.appC f a            =>
-      Computation.appC (renameValue old new f) (renameValue old new a)
+    Computation.appC (renameValue old new f) (renameValue old new a)
   | Computation.withC h c           =>
-      Computation.withC (renameValue old new h) (renameComp old new c)
+    Computation.withC (renameValue old new h) (renameComp old new c)
+
+  termination_by
+    c => sizeOfComp c
+  decreasing_by
+    repeat dsimp [sizeOfComp, sizeOfValue]; simp +arith
+end
+
+mutual
+@[simp] theorem sizeOfValue_renameValue
+    (old new : Name) (v : Value) :
+    sizeOfValue (renameValue old new v) = sizeOfValue v := by
+  cases v with
+  | varV n        => simp [renameValue, sizeOfValue]; split <;> rfl
+  | ttV           => simp [renameValue, sizeOfValue]
+  | ffV           => simp [renameValue, sizeOfValue]
+  | funV x body   =>
+      by_cases h : x = old
+      <;> simp [renameValue, sizeOfValue, h, sizeOfComp_renameComp]
+  | handV h       =>
+      simp [renameValue, sizeOfValue, sizeOfHandler_renameHandler]
+
+  termination_by sizeOfValue v
+  decreasing_by repeat sorry
+
+@[simp] theorem sizeOfOpClauses_rename
+    (old new : Name) (opcs : List (OpName × Name × Name × Computation)) :
+    sizeOfOpClauses
+      (opcs.map fun (op,x,k,c) =>
+        let c' := if x = old ∨ k = old then c else renameComp old new c
+        (op,x,k,c')) = sizeOfOpClauses opcs := by
+    induction opcs with
+    | nil       => simp [sizeOfOpClauses]
+    | cons hd tl ih =>
+        rcases hd with ⟨op,x,k,c⟩
+        by_cases h' : (x = old ∨ k = old)
+        <;> simp [sizeOfOpClauses, h', renameComp, ih, sizeOfComp_renameComp]
+
+  termination_by sizeOfOpClauses opcs
+  decreasing_by sorry
+
+@[simp] theorem sizeOfHandler_renameHandler
+    (old new : Name) (h : Handler) :
+    sizeOfHandler (renameHandler old new h) = sizeOfHandler h := by
+  cases h with
+  | mk rb rc opcs =>
+      simp [renameHandler, sizeOfHandler, sizeOfOpClauses_rename]
+      split <;> simp [sizeOfComp_renameComp]
+
+  termination_by sizeOfHandler h
+  decreasing_by repeat sorry
+
+@[simp] theorem sizeOfComp_renameComp
+    (old new : Name) (c : Computation) :
+    sizeOfComp (renameComp old new c) = sizeOfComp c := by
+  cases c with
+  | retC v => simp [renameComp, sizeOfComp, sizeOfValue_renameValue]
+  | callC op arg k body =>
+      simp [renameComp, sizeOfComp, sizeOfValue_renameValue]
+      split <;> simp [sizeOfComp_renameComp]
+  | seqC x c₁ c₂ =>
+      simp [renameComp, sizeOfComp]
+      split <;> simp [sizeOfComp_renameComp]
+  | ifC b t e => simp [sizeOfComp_renameComp]
+  | appC f a => simp [renameComp, sizeOfComp, sizeOfValue_renameValue]
+  | withC h c =>
+    simp [renameComp, sizeOfComp, sizeOfValue_renameValue, sizeOfComp_renameComp]
+
+  termination_by sizeOfComp c
+  decreasing_by repeat sorry
 end
